AwsCryptographyPrimitives/runtimes/java/src/main/smithy-generated/software/amazon/cryptography/primitives/model/GetHKDFProviderOutput.java
@@ -1,0 +1,61 @@
+// Copyright Amazon.com Inc. or its affiliates. All Rights Reserved.
+// SPDX-License-Identifier: Apache-2.0
+// Do not modify this file. This file is machine generated, and any changes to it will be overwritten.
+package software.amazon.cryptography.primitives.model;
+
+import java.util.Objects;
+
+public class GetHKDFProviderOutput {
+  private final HKDFProvider provider;
+
+  protected GetHKDFProviderOutput(BuilderImpl builder) {
+    this.provider = builder.provider();
+  }
+
+  public HKDFProvider provider() {
+    return this.provider;
+  }
+
+  public Builder toBuilder() {
+    return new BuilderImpl(this);
+  }
+
+  public static Builder builder() {
+    return new BuilderImpl();
+  }
+
+  public interface Builder {
+    Builder provider(HKDFProvider provider);
+
+    HKDFProvider provider();
+
+    GetHKDFProviderOutput build();
+  }
+
+  static class BuilderImpl implements Builder {
+    protected HKDFProvider provider;
+
+    protected BuilderImpl() {
+    }
+
+    protected BuilderImpl(GetHKDFProviderOutput model) {
+      this.provider = model.provider();
+    }
+
+    public Builder provider(HKDFProvider provider) {
+      this.provider = provider;
+      return this;
+    }
+
+    public HKDFProvider provider() {
+      return this.provider;
+    }
+
+    public GetHKDFProviderOutput build() {
+      if (Objects.isNull(this.provider()))  {
+        throw new IllegalArgumentException("Missing value for required field `provider`");
+      }
+      return new GetHKDFProviderOutput(this);
+    }
+  }
+}
