AwsCryptographyPrimitives/runtimes/java/src/main/smithy-generated/software/amazon/cryptography/primitives/model/HKDFProvider.java
@@ -1,0 +1,22 @@
+// Copyright Amazon.com Inc. or its affiliates. All Rights Reserved.
+// SPDX-License-Identifier: Apache-2.0
+// Do not modify this file. This file is machine generated, and any changes to it will be overwritten.
+package software.amazon.cryptography.primitives.model;
+
+public enum HKDFProvider {
+  ACCP_FIPS("ACCP_FIPS"),
+
+  ACCP_NOT_FIPS("ACCP_NOT_FIPS"),
+
+  MPL("MPL");
+
+  private final String value;
+
+  private HKDFProvider(String value) {
+    this.value = value;
+  }
+
+  public String toString() {
+    return String.valueOf(value);
+  }
+}
