AwsCryptographyPrimitives/runtimes/net/Generated/HKDFProvider.cs
@@ -1,0 +1,19 @@
+// Copyright Amazon.com Inc. or its affiliates. All Rights Reserved.
+// SPDX-License-Identifier: Apache-2.0
+// Do not modify this file. This file is machine generated, and any changes to it will be overwritten.
+using System;
+ using AWS.Cryptography.Primitives; namespace AWS.Cryptography.Primitives {
+ using Amazon.Runtime; public class HKDFProvider : ConstantClass {
+
+ 
+ public static readonly HKDFProvider ACCP_FIPS = new HKDFProvider ("ACCP_FIPS");
+ 
+ public static readonly HKDFProvider ACCP_NOT_FIPS = new HKDFProvider ("ACCP_NOT_FIPS");
+ 
+ public static readonly HKDFProvider MPL = new HKDFProvider ("MPL");
+ public static readonly  HKDFProvider [] Values =  {
+ ACCP_FIPS , ACCP_NOT_FIPS , MPL
+} ;
+ public HKDFProvider (string value) : base(value) {}
+}
+}
